coq

src/gen/main.c
@@ -1,0 +1,1627 @@
+#include "main.h"
+
+intptr_t idU_1; intptr_t idL_4; intptr_t rwlUU_7; intptr_t rwlUL_14;
+intptr_t rwlLU_21; intptr_t rwlLL_28; intptr_t rwrUU_35; intptr_t rwrUL_42;
+intptr_t rwrLU_49; intptr_t rwrLL_56; intptr_t sing_elimUU_63;
+intptr_t sing_elimUL_67; intptr_t sing_elimLU_71; intptr_t sing_elimLL_75;
+intptr_t not_79; intptr_t and_82; intptr_t or_87; intptr_t xor_92;
+intptr_t string_of_bool_98; intptr_t lte_103; intptr_t lt_113;
+intptr_t pred_118; intptr_t add_123; intptr_t sub_131; intptr_t mul_139;
+intptr_t div_147; intptr_t rem_167; intptr_t rconsUU_173;
+intptr_t rconsUL_184; intptr_t rconsLL_195; intptr_t free_listUU_206;
+intptr_t free_listUL_217; intptr_t free_listLL_228; intptr_t pow_239;
+intptr_t powm_253; intptr_t ord_269; intptr_t chr_272; intptr_t str_275;
+intptr_t strlen_279; intptr_t string_of_int_282; intptr_t sing_elimUU_310;
+intptr_t sing_elimUL_314; intptr_t sing_elimLU_318; intptr_t sing_elimLL_322;
+intptr_t free_streamU_326; intptr_t free_streamL_331;
+intptr_t uncons_streamU_336; intptr_t uncons_streamL_344;
+intptr_t nat_make_352; intptr_t proj1UUU_359; intptr_t proj1UUL_365;
+intptr_t proj1ULU_371; intptr_t proj1ULL_377; intptr_t proj1LUU_383;
+intptr_t proj1LUL_389; intptr_t proj1LLU_395; intptr_t proj1LLL_401;
+intptr_t proj2UUU_407; intptr_t proj2UUL_412; intptr_t proj2ULU_417;
+intptr_t proj2ULL_422; intptr_t proj2LUU_427; intptr_t proj2LUL_432;
+intptr_t proj2LLU_437; intptr_t proj2LLL_442; intptr_t my_apair0_447;
+intptr_t my_apair1_451; intptr_t __464;
+
+intptr_t fn0_idU_467(intptr_t A_2, intptr_t m_3) {
+  
+  
+  return m_3;
+}
+
+intptr_t fn1_idU_468(intptr_t* env) {
+  intptr_t A_2; intptr_t m_3; intptr_t x_469;
+  A_2 = env[1];
+  m_3 = env[2];
+  x_469 = fn0_idU_467(A_2, m_3);
+  return x_469;
+}
+
+intptr_t fn0_idL_470(intptr_t A_5, intptr_t m_6) {
+  
+  
+  return m_6;
+}
+
+intptr_t fn1_idL_471(intptr_t* env) {
+  intptr_t A_5; intptr_t m_6; intptr_t x_472;
+  A_5 = env[1];
+  m_6 = env[2];
+  x_472 = fn0_idL_470(A_5, m_6);
+  return x_472;
+}
+
+intptr_t fn0_rwlUU_473(intptr_t A_8, intptr_t m_9, intptr_t n_10, intptr_t B_11, intptr_t __12, intptr_t __13) {
+  
+  
+  return __13;
+}
+
+intptr_t fn1_rwlUU_474(intptr_t* env) {
+  intptr_t A_8; intptr_t m_9; intptr_t n_10; intptr_t B_11; intptr_t __12;
+  intptr_t __13; intptr_t x_475;
+  A_8 = env[1];
+  m_9 = env[2];
+  n_10 = env[3];
+  B_11 = env[4];
+  __12 = env[5];
+  __13 = env[6];
+  x_475 = fn0_rwlUU_473(A_8, m_9, n_10, B_11, __12, __13);
+  return x_475;
+}
+
+intptr_t fn0_rwlUL_476(intptr_t A_15, intptr_t m_16, intptr_t n_17, intptr_t B_18, intptr_t __19, intptr_t __20) {
+  
+  
+  return __20;
+}
+
+intptr_t fn1_rwlUL_477(intptr_t* env) {
+  intptr_t A_15; intptr_t m_16; intptr_t n_17; intptr_t B_18; intptr_t __19;
+  intptr_t __20; intptr_t x_478;
+  A_15 = env[1];
+  m_16 = env[2];
+  n_17 = env[3];
+  B_18 = env[4];
+  __19 = env[5];
+  __20 = env[6];
+  x_478 = fn0_rwlUL_476(A_15, m_16, n_17, B_18, __19, __20);
+  return x_478;
+}
+
+intptr_t fn0_rwlLU_479(intptr_t A_22, intptr_t m_23, intptr_t n_24, intptr_t B_25, intptr_t __26, intptr_t __27) {
+  
+  
+  return __27;
+}
+
+intptr_t fn1_rwlLU_480(intptr_t* env) {
+  intptr_t A_22; intptr_t m_23; intptr_t n_24; intptr_t B_25; intptr_t __26;
+  intptr_t __27; intptr_t x_481;
+  A_22 = env[1];
+  m_23 = env[2];
+  n_24 = env[3];
+  B_25 = env[4];
+  __26 = env[5];
+  __27 = env[6];
+  x_481 = fn0_rwlLU_479(A_22, m_23, n_24, B_25, __26, __27);
+  return x_481;
+}
+
+intptr_t fn0_rwlLL_482(intptr_t A_29, intptr_t m_30, intptr_t n_31, intptr_t B_32, intptr_t __33, intptr_t __34) {
+  
+  
+  return __34;
+}
+
+intptr_t fn1_rwlLL_483(intptr_t* env) {
+  intptr_t A_29; intptr_t m_30; intptr_t n_31; intptr_t B_32; intptr_t __33;
+  intptr_t __34; intptr_t x_484;
+  A_29 = env[1];
+  m_30 = env[2];
+  n_31 = env[3];
+  B_32 = env[4];
+  __33 = env[5];
+  __34 = env[6];
+  x_484 = fn0_rwlLL_482(A_29, m_30, n_31, B_32, __33, __34);
+  return x_484;
+}
+
+intptr_t fn0_rwrUU_485(intptr_t A_36, intptr_t m_37, intptr_t n_38, intptr_t B_39, intptr_t __40, intptr_t __41) {
+  
+  
+  return __41;
+}
+
+intptr_t fn1_rwrUU_486(intptr_t* env) {
+  intptr_t A_36; intptr_t m_37; intptr_t n_38; intptr_t B_39; intptr_t __40;
+  intptr_t __41; intptr_t x_487;
+  A_36 = env[1];
+  m_37 = env[2];
+  n_38 = env[3];
+  B_39 = env[4];
+  __40 = env[5];
+  __41 = env[6];
+  x_487 = fn0_rwrUU_485(A_36, m_37, n_38, B_39, __40, __41);
+  return x_487;
+}
+
+intptr_t fn0_rwrUL_488(intptr_t A_43, intptr_t m_44, intptr_t n_45, intptr_t B_46, intptr_t __47, intptr_t __48) {
+  
+  
+  return __48;
+}
+
+intptr_t fn1_rwrUL_489(intptr_t* env) {
+  intptr_t A_43; intptr_t m_44; intptr_t n_45; intptr_t B_46; intptr_t __47;
+  intptr_t __48; intptr_t x_490;
+  A_43 = env[1];
+  m_44 = env[2];
+  n_45 = env[3];
+  B_46 = env[4];
+  __47 = env[5];
+  __48 = env[6];
+  x_490 = fn0_rwrUL_488(A_43, m_44, n_45, B_46, __47, __48);
+  return x_490;
+}
+
+intptr_t fn0_rwrLU_491(intptr_t A_50, intptr_t m_51, intptr_t n_52, intptr_t B_53, intptr_t __54, intptr_t __55) {
+  
+  
+  return __55;
+}
+
+intptr_t fn1_rwrLU_492(intptr_t* env) {
+  intptr_t A_50; intptr_t m_51; intptr_t n_52; intptr_t B_53; intptr_t __54;
+  intptr_t __55; intptr_t x_493;
+  A_50 = env[1];
+  m_51 = env[2];
+  n_52 = env[3];
+  B_53 = env[4];
+  __54 = env[5];
+  __55 = env[6];
+  x_493 = fn0_rwrLU_491(A_50, m_51, n_52, B_53, __54, __55);
+  return x_493;
+}
+
+intptr_t fn0_rwrLL_494(intptr_t A_57, intptr_t m_58, intptr_t n_59, intptr_t B_60, intptr_t __61, intptr_t __62) {
+  
+  
+  return __62;
+}
+
+intptr_t fn1_rwrLL_495(intptr_t* env) {
+  intptr_t A_57; intptr_t m_58; intptr_t n_59; intptr_t B_60; intptr_t __61;
+  intptr_t __62; intptr_t x_496;
+  A_57 = env[1];
+  m_58 = env[2];
+  n_59 = env[3];
+  B_60 = env[4];
+  __61 = env[5];
+  __62 = env[6];
+  x_496 = fn0_rwrLL_494(A_57, m_58, n_59, B_60, __61, __62);
+  return x_496;
+}
+
+intptr_t fn0_sing_elimUU_497(intptr_t A_64, intptr_t x_65, intptr_t __66) {
+  
+  
+  return __66;
+}
+
+intptr_t fn1_sing_elimUU_498(intptr_t* env) {
+  intptr_t A_64; intptr_t x_65; intptr_t __66; intptr_t x_499;
+  A_64 = env[1];
+  x_65 = env[2];
+  __66 = env[3];
+  x_499 = fn0_sing_elimUU_497(A_64, x_65, __66);
+  return x_499;
+}
+
+intptr_t fn0_sing_elimUL_500(intptr_t A_68, intptr_t x_69, intptr_t __70) {
+  
+  
+  return __70;
+}
+
+intptr_t fn1_sing_elimUL_501(intptr_t* env) {
+  intptr_t A_68; intptr_t x_69; intptr_t __70; intptr_t x_502;
+  A_68 = env[1];
+  x_69 = env[2];
+  __70 = env[3];
+  x_502 = fn0_sing_elimUL_500(A_68, x_69, __70);
+  return x_502;
+}
+
+intptr_t fn0_sing_elimLU_503(intptr_t A_72, intptr_t x_73, intptr_t __74) {
+  
+  absurd();
+  return nothing;
+}
+
+intptr_t fn1_sing_elimLU_504(intptr_t* env) {
+  intptr_t A_72; intptr_t x_73; intptr_t __74; intptr_t x_505;
+  A_72 = env[1];
+  x_73 = env[2];
+  __74 = env[3];
+  x_505 = fn0_sing_elimLU_503(A_72, x_73, __74);
+  return x_505;
+}
+
+intptr_t fn0_sing_elimLL_506(intptr_t A_76, intptr_t x_77, intptr_t __78) {
+  
+  
+  return __78;
+}
+
+intptr_t fn1_sing_elimLL_507(intptr_t* env) {
+  intptr_t A_76; intptr_t x_77; intptr_t __78; intptr_t x_508;
+  A_76 = env[1];
+  x_77 = env[2];
+  __78 = env[3];
+  x_508 = fn0_sing_elimLL_506(A_76, x_77, __78);
+  return x_508;
+}
+
+intptr_t fn0_not_509(intptr_t __80) {
+  intptr_t x_81;
+  switch(__80){
+    case 4: //true_4
+      x_81 = 5;
+      break;
+    case 5: //false_5
+      x_81 = 4;
+      break;
+  }
+  return x_81;
+}
+
+intptr_t fn1_not_510(intptr_t* env) {
+  intptr_t __80; intptr_t x_511;
+  __80 = env[1];
+  x_511 = fn0_not_509(__80);
+  return x_511;
+}
+
+intptr_t fn0_and_512(intptr_t __83, intptr_t __84) {
+  intptr_t x_85; intptr_t x_86;
+  switch(__83){
+    case 4: //true_4
+      switch(__84){
+        case 4: //true_4
+          x_86 = 4;
+          break;
+        case 5: //false_5
+          x_86 = 5;
+          break;
+      }
+      x_85 = x_86;
+      break;
+    case 5: //false_5
+      x_85 = 5;
+      break;
+  }
+  return x_85;
+}
+
+intptr_t fn1_and_513(intptr_t* env) {
+  intptr_t __83; intptr_t __84; intptr_t x_514;
+  __83 = env[1];
+  __84 = env[2];
+  x_514 = fn0_and_512(__83, __84);
+  return x_514;
+}
+
+intptr_t fn0_or_515(intptr_t __88, intptr_t __89) {
+  intptr_t x_90; intptr_t x_91;
+  switch(__88){
+    case 4: //true_4
+      x_90 = 4;
+      break;
+    case 5: //false_5
+      switch(__89){
+        case 4: //true_4
+          x_91 = 4;
+          break;
+        case 5: //false_5
+          x_91 = 5;
+          break;
+      }
+      x_90 = x_91;
+      break;
+  }
+  return x_90;
+}
+
+intptr_t fn1_or_516(intptr_t* env) {
+  intptr_t __88; intptr_t __89; intptr_t x_517;
+  __88 = env[1];
+  __89 = env[2];
+  x_517 = fn0_or_515(__88, __89);
+  return x_517;
+}
+
+intptr_t fn0_xor_518(intptr_t __93, intptr_t __94) {
+  intptr_t x_95; intptr_t x_96; intptr_t x_97;
+  switch(__93){
+    case 4: //true_4
+      switch(__94){
+        case 4: //true_4
+          x_96 = 5;
+          break;
+        case 5: //false_5
+          x_96 = 4;
+          break;
+      }
+      x_95 = x_96;
+      break;
+    case 5: //false_5
+      switch(__94){
+        case 4: //true_4
+          x_97 = 4;
+          break;
+        case 5: //false_5
+          x_97 = 5;
+          break;
+      }
+      x_95 = x_97;
+      break;
+  }
+  return x_95;
+}
+
+intptr_t fn1_xor_519(intptr_t* env) {
+  intptr_t __93; intptr_t __94; intptr_t x_520;
+  __93 = env[1];
+  __94 = env[2];
+  x_520 = fn0_xor_518(__93, __94);
+  return x_520;
+}
+
+intptr_t fn0_string_of_bool_521(intptr_t __99) {
+  intptr_t x_100; intptr_t x_101; intptr_t x_102;
+  switch(__99){
+    case 4: //true_4
+      x_101 = __str__("true");
+      x_100 = x_101;
+      break;
+    case 5: //false_5
+      x_102 = __str__("false");
+      x_100 = x_102;
+      break;
+  }
+  return x_100;
+}
+
+intptr_t fn1_string_of_bool_522(intptr_t* env) {
+  intptr_t __99; intptr_t x_523;
+  __99 = env[1];
+  x_523 = fn0_string_of_bool_521(__99);
+  return x_523;
+}
+
+intptr_t fn0_lte_524(intptr_t __104, intptr_t __105) {
+  intptr_t x_106; intptr_t x_107; intptr_t n_108; intptr_t x_109;
+  intptr_t x_110; intptr_t n_111; intptr_t x_112;
+  switch(__104){
+    case 6: //zero_6
+      x_106 = 4;
+      break;
+    default:
+      n_108 = getbox(__104, 0);
+      switch(__105){
+        case 6: //zero_6
+          x_109 = 5;
+          break;
+        default:
+          n_111 = getbox(__105, 0);
+          x_112 = fn0_lte_524(n_108, n_111);
+          x_110 = x_112;
+          x_109 = x_110;
+          break;
+      }
+      x_107 = x_109;
+      x_106 = x_107;
+      break;
+  }
+  return x_106;
+}
+
+intptr_t fn1_lte_525(intptr_t* env) {
+  intptr_t __104; intptr_t __105; intptr_t x_526;
+  __104 = env[1];
+  __105 = env[2];
+  x_526 = fn0_lte_524(__104, __105);
+  return x_526;
+}
+
+intptr_t fn0_lt_527(intptr_t x_114, intptr_t y_115) {
+  intptr_t x_116; intptr_t x_117;
+  x_117 = mkbox(7, 1); //succ_7
+  setbox(x_117, x_114, 0);
+  x_116 = fn0_lte_524(x_117, y_115);
+  return x_116;
+}
+
+intptr_t fn1_lt_528(intptr_t* env) {
+  intptr_t x_114; intptr_t y_115; intptr_t x_529;
+  x_114 = env[1];
+  y_115 = env[2];
+  x_529 = fn0_lt_527(x_114, y_115);
+  return x_529;
+}
+
+intptr_t fn0_pred_530(intptr_t __119) {
+  intptr_t x_120; intptr_t x_121; intptr_t n_122;
+  switch(__119){
+    case 6: //zero_6
+      x_120 = 6;
+      break;
+    default:
+      n_122 = getbox(__119, 0);
+      x_121 = n_122;
+      x_120 = x_121;
+      break;
+  }
+  return x_120;
+}
+
+intptr_t fn1_pred_531(intptr_t* env) {
+  intptr_t __119; intptr_t x_532;
+  __119 = env[1];
+  x_532 = fn0_pred_530(__119);
+  return x_532;
+}
+
+intptr_t fn0_add_533(intptr_t __124, intptr_t __125) {
+  intptr_t x_126; intptr_t x_127; intptr_t n_128; intptr_t x_129;
+  intptr_t x_130;
+  switch(__124){
+    case 6: //zero_6
+      x_126 = __125;
+      break;
+    default:
+      n_128 = getbox(__124, 0);
+      x_129 = fn0_add_533(n_128, __125);
+      x_130 = mkbox(7, 1); //succ_7
+      setbox(x_130, x_129, 0);
+      x_127 = x_130;
+      x_126 = x_127;
+      break;
+  }
+  return x_126;
+}
+
+intptr_t fn1_add_534(intptr_t* env) {
+  intptr_t __124; intptr_t __125; intptr_t x_535;
+  __124 = env[1];
+  __125 = env[2];
+  x_535 = fn0_add_533(__124, __125);
+  return x_535;
+}
+
+intptr_t fn0_sub_536(intptr_t __132, intptr_t __133) {
+  intptr_t x_134; intptr_t x_135; intptr_t n_136; intptr_t x_137;
+  intptr_t x_138;
+  switch(__133){
+    case 6: //zero_6
+      x_134 = __132;
+      break;
+    default:
+      n_136 = getbox(__133, 0);
+      x_138 = fn0_pred_530(__132);
+      x_137 = fn0_sub_536(x_138, n_136);
+      x_135 = x_137;
+      x_134 = x_135;
+      break;
+  }
+  return x_134;
+}
+
+intptr_t fn1_sub_537(intptr_t* env) {
+  intptr_t __132; intptr_t __133; intptr_t x_538;
+  __132 = env[1];
+  __133 = env[2];
+  x_538 = fn0_sub_536(__132, __133);
+  return x_538;
+}
+
+intptr_t fn0_mul_539(intptr_t __140, intptr_t __141) {
+  intptr_t x_142; intptr_t x_143; intptr_t n_144; intptr_t x_145;
+  intptr_t x_146;
+  switch(__140){
+    case 6: //zero_6
+      x_142 = 6;
+      break;
+    default:
+      n_144 = getbox(__140, 0);
+      x_146 = fn0_mul_539(n_144, __141);
+      x_145 = fn0_add_533(__141, x_146);
+      x_143 = x_145;
+      x_142 = x_143;
+      break;
+  }
+  return x_142;
+}
+
+intptr_t fn1_mul_540(intptr_t* env) {
+  intptr_t __140; intptr_t __141; intptr_t x_541;
+  __140 = env[1];
+  __141 = env[2];
+  x_541 = fn0_mul_539(__140, __141);
+  return x_541;
+}
+
+intptr_t fn0_div_542(intptr_t x_148, intptr_t y_149) {
+  intptr_t x_150; intptr_t x_151; intptr_t loop_152; intptr_t x_153;
+  intptr_t x_166; intptr_t x_548; intptr_t x_549;
+  x_151 = fn0_lt_527(x_148, y_149);
+  switch(x_151){
+    case 4: //true_4
+      x_150 = 6;
+      break;
+    case 5: //false_5
+      x_153 = mkclo(fn1_loop_544, 2, 2);
+      setclo(x_153, pred_118, 1);
+      setclo(x_153, sub_131, 2);
+      loop_152 = x_153;
+      x_548 = appc(loop_152, x_148);
+      x_549 = appc(x_548, y_149);
+      x_166 = x_549;
+      x_150 = x_166;
+      break;
+  }
+  return x_150;
+}
+
+intptr_t fn1_div_543(intptr_t* env) {
+  intptr_t x_148; intptr_t y_149; intptr_t x_551;
+  x_148 = env[1];
+  y_149 = env[2];
+  x_551 = fn0_div_542(x_148, y_149);
+  return x_551;
+}
+
+intptr_t fn0_rem_552(intptr_t x_168, intptr_t y_169) {
+  intptr_t x_170; intptr_t x_171; intptr_t x_172;
+  x_172 = fn0_div_542(x_168, y_169);
+  x_171 = fn0_mul_539(x_172, y_169);
+  x_170 = fn0_sub_536(x_168, x_171);
+  return x_170;
+}
+
+intptr_t fn1_rem_553(intptr_t* env) {
+  intptr_t x_168; intptr_t y_169; intptr_t x_554;
+  x_168 = env[1];
+  y_169 = env[2];
+  x_554 = fn0_rem_552(x_168, y_169);
+  return x_554;
+}
+
+intptr_t fn0_rconsUU_555(intptr_t A_174, intptr_t __175, intptr_t __176) {
+  intptr_t x_177; intptr_t x_178; intptr_t x_179; intptr_t hd_180;
+  intptr_t tl_181; intptr_t x_182; intptr_t x_183;
+  switch(__175){
+    case 38: //nilUU_38
+      x_178 = mkbox(39, 2); //consUU_39
+      setbox(x_178, __176, 0);
+      setbox(x_178, 38, 1);
+      x_177 = x_178;
+      break;
+    default:
+      hd_180 = getbox(__175, 0);
+      tl_181 = getbox(__175, 1);
+      x_182 = fn0_rconsUU_555(nothing, tl_181, __176);
+      x_183 = mkbox(39, 2); //consUU_39
+      setbox(x_183, hd_180, 0);
+      setbox(x_183, x_182, 1);
+      x_179 = x_183;
+      x_177 = x_179;
+      break;
+  }
+  return x_177;
+}
+
+intptr_t fn1_rconsUU_556(intptr_t* env) {
+  intptr_t A_174; intptr_t __175; intptr_t __176; intptr_t x_557;
+  A_174 = env[1];
+  __175 = env[2];
+  __176 = env[3];
+  x_557 = fn0_rconsUU_555(A_174, __175, __176);
+  return x_557;
+}
+
+intptr_t fn0_rconsUL_558(intptr_t A_185, intptr_t __186, intptr_t __187) {
+  intptr_t x_188; intptr_t x_189; intptr_t x_190; intptr_t hd_191;
+  intptr_t tl_192; intptr_t x_193; intptr_t x_194;
+  switch(__186){
+    case 36: //nilUL_36
+      x_189 = mkbox(37, 2); //consUL_37
+      setbox(x_189, __187, 0);
+      setbox(x_189, 36, 1);
+      x_188 = x_189;
+      break;
+    default:
+      hd_191 = getbox(__186, 0);
+      tl_192 = getbox(__186, 1);
+      x_193 = fn0_rconsUL_558(nothing, tl_192, __187);
+      x_194 = rebox(__186, 37); //consUL_37
+      setbox(x_194, hd_191, 0);
+      setbox(x_194, x_193, 1);
+      x_190 = x_194;
+      x_188 = x_190;
+      break;
+  }
+  return x_188;
+}
+
+intptr_t fn1_rconsUL_559(intptr_t* env) {
+  intptr_t A_185; intptr_t __186; intptr_t __187; intptr_t x_560;
+  A_185 = env[1];
+  __186 = env[2];
+  __187 = env[3];
+  x_560 = fn0_rconsUL_558(A_185, __186, __187);
+  return x_560;
+}
+
+intptr_t fn0_rconsLL_561(intptr_t A_196, intptr_t __197, intptr_t __198) {
+  intptr_t x_199; intptr_t x_200; intptr_t x_201; intptr_t hd_202;
+  intptr_t tl_203; intptr_t x_204; intptr_t x_205;
+  switch(__197){
+    case 32: //nilLL_32
+      x_200 = mkbox(33, 2); //consLL_33
+      setbox(x_200, __198, 0);
+      setbox(x_200, 32, 1);
+      x_199 = x_200;
+      break;
+    default:
+      hd_202 = getbox(__197, 0);
+      tl_203 = getbox(__197, 1);
+      x_204 = fn0_rconsLL_561(nothing, tl_203, __198);
+      x_205 = rebox(__197, 33); //consLL_33
+      setbox(x_205, hd_202, 0);
+      setbox(x_205, x_204, 1);
+      x_201 = x_205;
+      x_199 = x_201;
+      break;
+  }
+  return x_199;
+}
+
+intptr_t fn1_rconsLL_562(intptr_t* env) {
+  intptr_t A_196; intptr_t __197; intptr_t __198; intptr_t x_563;
+  A_196 = env[1];
+  __197 = env[2];
+  __198 = env[3];
+  x_563 = fn0_rconsLL_561(A_196, __197, __198);
+  return x_563;
+}
+
+intptr_t fn0_free_listUU_564(intptr_t A_207, intptr_t f_208, intptr_t __209) {
+  intptr_t x_210; intptr_t x_211; intptr_t hd_212; intptr_t tl_213;
+  intptr_t __214; intptr_t x_215; intptr_t x_216; intptr_t x_566;
+  switch(__209){
+    case 38: //nilUU_38
+      x_210 = 27;
+      break;
+    default:
+      hd_212 = getbox(__209, 0);
+      tl_213 = getbox(__209, 1);
+      x_566 = appc(f_208, hd_212);
+      x_215 = x_566;
+      __214 = x_215;
+      x_216 = fn0_free_listUU_564(nothing, f_208, tl_213);
+      x_211 = x_216;
+      x_210 = x_211;
+      break;
+  }
+  return x_210;
+}
+
+intptr_t fn1_free_listUU_565(intptr_t* env) {
+  intptr_t A_207; intptr_t f_208; intptr_t __209; intptr_t x_568;
+  A_207 = env[1];
+  f_208 = env[2];
+  __209 = env[3];
+  x_568 = fn0_free_listUU_564(A_207, f_208, __209);
+  return x_568;
+}
+
+intptr_t fn0_free_listUL_569(intptr_t A_218, intptr_t f_219, intptr_t __220) {
+  intptr_t x_221; intptr_t x_222; intptr_t hd_223; intptr_t tl_224;
+  intptr_t __225; intptr_t x_226; intptr_t x_227; intptr_t x_571;
+  switch(__220){
+    case 36: //nilUL_36
+      x_221 = 27;
+      break;
+    default:
+      hd_223 = getbox(__220, 0);
+      tl_224 = getbox(__220, 1);
+      x_571 = appc(f_219, hd_223);
+      x_226 = x_571;
+      __225 = x_226;
+      x_227 = fn0_free_listUL_569(nothing, f_219, tl_224);
+      x_222 = x_227;
+      ffree(__220);
+      x_221 = x_222;
+      break;
+  }
+  return x_221;
+}
+
+intptr_t fn1_free_listUL_570(intptr_t* env) {
+  intptr_t A_218; intptr_t f_219; intptr_t __220; intptr_t x_573;
+  A_218 = env[1];
+  f_219 = env[2];
+  __220 = env[3];
+  x_573 = fn0_free_listUL_569(A_218, f_219, __220);
+  return x_573;
+}
+
+intptr_t fn0_free_listLL_574(intptr_t A_229, intptr_t f_230, intptr_t __231) {
+  intptr_t x_232; intptr_t x_233; intptr_t hd_234; intptr_t tl_235;
+  intptr_t __236; intptr_t x_237; intptr_t x_238; intptr_t x_576;
+  switch(__231){
+    case 32: //nilLL_32
+      x_232 = 27;
+      break;
+    default:
+      hd_234 = getbox(__231, 0);
+      tl_235 = getbox(__231, 1);
+      x_576 = appc(f_230, hd_234);
+      x_237 = x_576;
+      __236 = x_237;
+      x_238 = fn0_free_listLL_574(nothing, f_230, tl_235);
+      x_233 = x_238;
+      ffree(__231);
+      x_232 = x_233;
+      break;
+  }
+  return x_232;
+}
+
+intptr_t fn1_free_listLL_575(intptr_t* env) {
+  intptr_t A_229; intptr_t f_230; intptr_t __231; intptr_t x_578;
+  A_229 = env[1];
+  f_230 = env[2];
+  __231 = env[3];
+  x_578 = fn0_free_listLL_574(A_229, f_230, __231);
+  return x_578;
+}
+
+intptr_t fn0_pow_579(intptr_t x_240, intptr_t y_241) {
+  intptr_t loop_242; intptr_t x_243; intptr_t x_252; intptr_t x_585;
+  intptr_t x_586;
+  x_243 = mkclo(fn1_loop_581, 1, 2);
+  setclo(x_243, x_240, 1);
+  loop_242 = x_243;
+  x_585 = appc(loop_242, 1);
+  x_586 = appc(x_585, y_241);
+  x_252 = x_586;
+  return x_252;
+}
+
+intptr_t fn1_pow_580(intptr_t* env) {
+  intptr_t x_240; intptr_t y_241; intptr_t x_588;
+  x_240 = env[1];
+  y_241 = env[2];
+  x_588 = fn0_pow_579(x_240, y_241);
+  return x_588;
+}
+
+intptr_t fn0_powm_589(intptr_t x_254, intptr_t y_255, intptr_t m_256) {
+  intptr_t loop_257; intptr_t x_258; intptr_t x_268; intptr_t x_595;
+  intptr_t x_596;
+  x_258 = mkclo(fn1_loop_591, 2, 2);
+  setclo(x_258, x_254, 1);
+  setclo(x_258, m_256, 2);
+  loop_257 = x_258;
+  x_595 = appc(loop_257, 1);
+  x_596 = appc(x_595, y_255);
+  x_268 = x_596;
+  return x_268;
+}
+
+intptr_t fn1_powm_590(intptr_t* env) {
+  intptr_t x_254; intptr_t y_255; intptr_t m_256; intptr_t x_598;
+  x_254 = env[1];
+  y_255 = env[2];
+  m_256 = env[3];
+  x_598 = fn0_powm_589(x_254, y_255, m_256);
+  return x_598;
+}
+
+intptr_t fn0_ord_599(intptr_t c_270) {
+  intptr_t x_271;
+  x_271 = __ord__(c_270);
+  return x_271;
+}
+
+intptr_t fn1_ord_600(intptr_t* env) {
+  intptr_t c_270; intptr_t x_601;
+  c_270 = env[1];
+  x_601 = fn0_ord_599(c_270);
+  return x_601;
+}
+
+intptr_t fn0_chr_602(intptr_t i_273) {
+  intptr_t x_274;
+  x_274 = __chr__(i_273);
+  return x_274;
+}
+
+intptr_t fn1_chr_603(intptr_t* env) {
+  intptr_t i_273; intptr_t x_604;
+  i_273 = env[1];
+  x_604 = fn0_chr_602(i_273);
+  return x_604;
+}
+
+intptr_t fn0_str_605(intptr_t c_276) {
+  intptr_t x_277; intptr_t x_278;
+  x_278 = __str__("");
+  x_277 = __push__(x_278, c_276);
+  return x_277;
+}
+
+intptr_t fn1_str_606(intptr_t* env) {
+  intptr_t c_276; intptr_t x_607;
+  c_276 = env[1];
+  x_607 = fn0_str_605(c_276);
+  return x_607;
+}
+
+intptr_t fn0_strlen_608(intptr_t s_280) {
+  intptr_t x_281;
+  x_281 = __size__(s_280);
+  return x_281;
+}
+
+intptr_t fn1_strlen_609(intptr_t* env) {
+  intptr_t s_280; intptr_t x_610;
+  s_280 = env[1];
+  x_610 = fn0_strlen_608(s_280);
+  return x_610;
+}
+
+intptr_t fn0_string_of_int_611(intptr_t i_283) {
+  intptr_t aux_284; intptr_t x_285; intptr_t x_303; intptr_t x_304;
+  intptr_t x_305; intptr_t x_306; intptr_t x_307; intptr_t x_308;
+  intptr_t x_309; intptr_t x_616; intptr_t x_618;
+  x_285 = mkclo(fn1_aux_613, 3, 1);
+  setclo(x_285, ord_269, 1);
+  setclo(x_285, chr_272, 2);
+  setclo(x_285, str_275, 3);
+  aux_284 = x_285;
+  x_304 = __lte__(0, i_283);
+  switch(x_304){
+    case 4: //true_4
+      x_616 = appc(aux_284, i_283);
+      x_305 = x_616;
+      x_303 = x_305;
+      break;
+    case 5: //false_5
+      x_307 = __str__("~");
+      x_309 = __neg__(i_283);
+      x_618 = appc(aux_284, x_309);
+      x_308 = x_618;
+      x_306 = __cat__(x_307, x_308);
+      x_303 = x_306;
+      break;
+  }
+  return x_303;
+}
+
+intptr_t fn1_string_of_int_612(intptr_t* env) {
+  intptr_t i_283; intptr_t x_620;
+  i_283 = env[1];
+  x_620 = fn0_string_of_int_611(i_283);
+  return x_620;
+}
+
+intptr_t fn0_sing_elimUU_621(intptr_t A_311, intptr_t x_312, intptr_t __313) {
+  
+  
+  return __313;
+}
+
+intptr_t fn1_sing_elimUU_622(intptr_t* env) {
+  intptr_t A_311; intptr_t x_312; intptr_t __313; intptr_t x_623;
+  A_311 = env[1];
+  x_312 = env[2];
+  __313 = env[3];
+  x_623 = fn0_sing_elimUU_621(A_311, x_312, __313);
+  return x_623;
+}
+
+intptr_t fn0_sing_elimUL_624(intptr_t A_315, intptr_t x_316, intptr_t __317) {
+  
+  
+  return __317;
+}
+
+intptr_t fn1_sing_elimUL_625(intptr_t* env) {
+  intptr_t A_315; intptr_t x_316; intptr_t __317; intptr_t x_626;
+  A_315 = env[1];
+  x_316 = env[2];
+  __317 = env[3];
+  x_626 = fn0_sing_elimUL_624(A_315, x_316, __317);
+  return x_626;
+}
+
+intptr_t fn0_sing_elimLU_627(intptr_t A_319, intptr_t x_320, intptr_t __321) {
+  
+  absurd();
+  return nothing;
+}
+
+intptr_t fn1_sing_elimLU_628(intptr_t* env) {
+  intptr_t A_319; intptr_t x_320; intptr_t __321; intptr_t x_629;
+  A_319 = env[1];
+  x_320 = env[2];
+  __321 = env[3];
+  x_629 = fn0_sing_elimLU_627(A_319, x_320, __321);
+  return x_629;
+}
+
+intptr_t fn0_sing_elimLL_630(intptr_t A_323, intptr_t x_324, intptr_t __325) {
+  
+  
+  return __325;
+}
+
+intptr_t fn1_sing_elimLL_631(intptr_t* env) {
+  intptr_t A_323; intptr_t x_324; intptr_t __325; intptr_t x_632;
+  A_323 = env[1];
+  x_324 = env[2];
+  __325 = env[3];
+  x_632 = fn0_sing_elimLL_630(A_323, x_324, __325);
+  return x_632;
+}
+
+intptr_t fn0_free_streamU_633(intptr_t A_327, intptr_t st_328) {
+  intptr_t x_329; intptr_t x_330; intptr_t x_635;
+  x_635 = appc(st_328, 17);
+  ffree(st_328);
+  x_330 = x_635;
+  switch(x_330){
+    case 26: //ttL_26
+      x_329 = 27;
+      break;
+  }
+  return x_329;
+}
+
+intptr_t fn1_free_streamU_634(intptr_t* env) {
+  intptr_t A_327; intptr_t st_328; intptr_t x_637;
+  A_327 = env[1];
+  st_328 = env[2];
+  x_637 = fn0_free_streamU_633(A_327, st_328);
+  return x_637;
+}
+
+intptr_t fn0_free_streamL_638(intptr_t A_332, intptr_t st_333) {
+  intptr_t x_334; intptr_t x_335; intptr_t x_640;
+  x_640 = appc(st_333, 17);
+  ffree(st_333);
+  x_335 = x_640;
+  switch(x_335){
+    case 26: //ttL_26
+      x_334 = 27;
+      break;
+  }
+  return x_334;
+}
+
+intptr_t fn1_free_streamL_639(intptr_t* env) {
+  intptr_t A_332; intptr_t st_333; intptr_t x_642;
+  A_332 = env[1];
+  st_333 = env[2];
+  x_642 = fn0_free_streamL_638(A_332, st_333);
+  return x_642;
+}
+
+intptr_t fn0_uncons_streamU_643(intptr_t A_337, intptr_t st_338) {
+  intptr_t x_339; intptr_t x_340; intptr_t hd_341; intptr_t tl_342;
+  intptr_t x_343; intptr_t x_645;
+  x_645 = appc(st_338, 16);
+  ffree(st_338);
+  x_340 = x_645;
+  hd_341 = getbox(x_340, 0);
+  tl_342 = getbox(x_340, 1);
+  x_343 = rebox(x_340, 50); //ex1UL_50
+  setbox(x_343, hd_341, 0);
+  setbox(x_343, tl_342, 1);
+  x_339 = x_343;
+  return x_339;
+}
+
+intptr_t fn1_uncons_streamU_644(intptr_t* env) {
+  intptr_t A_337; intptr_t st_338; intptr_t x_647;
+  A_337 = env[1];
+  st_338 = env[2];
+  x_647 = fn0_uncons_streamU_643(A_337, st_338);
+  return x_647;
+}
+
+intptr_t fn0_uncons_streamL_648(intptr_t A_345, intptr_t st_346) {
+  intptr_t x_347; intptr_t x_348; intptr_t hd_349; intptr_t tl_350;
+  intptr_t x_351; intptr_t x_650;
+  x_650 = appc(st_346, 16);
+  ffree(st_346);
+  x_348 = x_650;
+  hd_349 = getbox(x_348, 0);
+  tl_350 = getbox(x_348, 1);
+  x_351 = rebox(x_348, 48); //ex1LL_48
+  setbox(x_351, hd_349, 0);
+  setbox(x_351, tl_350, 1);
+  x_347 = x_351;
+  return x_347;
+}
+
+intptr_t fn1_uncons_streamL_649(intptr_t* env) {
+  intptr_t A_345; intptr_t st_346; intptr_t x_652;
+  A_345 = env[1];
+  st_346 = env[2];
+  x_652 = fn0_uncons_streamL_648(A_345, st_346);
+  return x_652;
+}
+
+intptr_t fn0_nat_make_653(intptr_t n_353, intptr_t x_354) {
+  intptr_t x_355; intptr_t x_356; intptr_t x_357; intptr_t x_358;
+  intptr_t x_655;
+  switch(x_354){
+    case 16: //next_16
+      x_357 = mkbox(7, 1); //succ_7
+      setbox(x_357, n_353, 0);
+      x_655 = appc(nat_make_352, x_357);
+      x_356 = x_655;
+      x_358 = mkbox(55, 2); //stream_consU_55
+      setbox(x_358, n_353, 0);
+      setbox(x_358, x_356, 1);
+      x_355 = x_358;
+      break;
+    case 17: //free_17
+      x_355 = 26;
+      break;
+  }
+  return x_355;
+}
+
+intptr_t fn1_nat_make_654(intptr_t* env) {
+  intptr_t n_353; intptr_t x_354; intptr_t x_657;
+  n_353 = env[1];
+  x_354 = env[2];
+  x_657 = fn0_nat_make_653(n_353, x_354);
+  return x_657;
+}
+
+intptr_t fn0_proj1UUU_658(intptr_t A_360, intptr_t B_361, intptr_t __362) {
+  intptr_t x_363; intptr_t x_364; intptr_t x_660;
+  x_660 = appc(__362, 4);
+  x_364 = x_660;
+  x_363 = fn0_sing_elimUL_624(nothing, nothing, x_364);
+  return x_363;
+}
+
+intptr_t fn1_proj1UUU_659(intptr_t* env) {
+  intptr_t A_360; intptr_t B_361; intptr_t __362; intptr_t x_662;
+  A_360 = env[1];
+  B_361 = env[2];
+  __362 = env[3];
+  x_662 = fn0_proj1UUU_658(A_360, B_361, __362);
+  return x_662;
+}
+
+intptr_t fn0_proj1UUL_663(intptr_t A_366, intptr_t B_367, intptr_t __368) {
+  intptr_t x_369; intptr_t x_370; intptr_t x_665;
+  x_665 = appc(__368, 4);
+  ffree(__368);
+  x_370 = x_665;
+  x_369 = fn0_sing_elimUL_624(nothing, nothing, x_370);
+  return x_369;
+}
+
+intptr_t fn1_proj1UUL_664(intptr_t* env) {
+  intptr_t A_366; intptr_t B_367; intptr_t __368; intptr_t x_667;
+  A_366 = env[1];
+  B_367 = env[2];
+  __368 = env[3];
+  x_667 = fn0_proj1UUL_663(A_366, B_367, __368);
+  return x_667;
+}
+
+intptr_t fn0_proj1ULU_668(intptr_t A_372, intptr_t B_373, intptr_t __374) {
+  intptr_t x_375; intptr_t x_376; intptr_t x_670;
+  x_670 = appc(__374, 4);
+  x_376 = x_670;
+  x_375 = fn0_sing_elimUL_624(nothing, nothing, x_376);
+  return x_375;
+}
+
+intptr_t fn1_proj1ULU_669(intptr_t* env) {
+  intptr_t A_372; intptr_t B_373; intptr_t __374; intptr_t x_672;
+  A_372 = env[1];
+  B_373 = env[2];
+  __374 = env[3];
+  x_672 = fn0_proj1ULU_668(A_372, B_373, __374);
+  return x_672;
+}
+
+intptr_t fn0_proj1ULL_673(intptr_t A_378, intptr_t B_379, intptr_t __380) {
+  intptr_t x_381; intptr_t x_382; intptr_t x_675;
+  x_675 = appc(__380, 4);
+  ffree(__380);
+  x_382 = x_675;
+  x_381 = fn0_sing_elimUL_624(nothing, nothing, x_382);
+  return x_381;
+}
+
+intptr_t fn1_proj1ULL_674(intptr_t* env) {
+  intptr_t A_378; intptr_t B_379; intptr_t __380; intptr_t x_677;
+  A_378 = env[1];
+  B_379 = env[2];
+  __380 = env[3];
+  x_677 = fn0_proj1ULL_673(A_378, B_379, __380);
+  return x_677;
+}
+
+intptr_t fn0_proj1LUU_678(intptr_t A_384, intptr_t B_385, intptr_t __386) {
+  intptr_t x_387; intptr_t x_388; intptr_t x_680;
+  x_680 = appc(__386, 4);
+  x_388 = x_680;
+  x_387 = fn0_sing_elimLL_630(nothing, nothing, x_388);
+  return x_387;
+}
+
+intptr_t fn1_proj1LUU_679(intptr_t* env) {
+  intptr_t A_384; intptr_t B_385; intptr_t __386; intptr_t x_682;
+  A_384 = env[1];
+  B_385 = env[2];
+  __386 = env[3];
+  x_682 = fn0_proj1LUU_678(A_384, B_385, __386);
+  return x_682;
+}
+
+intptr_t fn0_proj1LUL_683(intptr_t A_390, intptr_t B_391, intptr_t __392) {
+  intptr_t x_393; intptr_t x_394; intptr_t x_685;
+  x_685 = appc(__392, 4);
+  ffree(__392);
+  x_394 = x_685;
+  x_393 = fn0_sing_elimLL_630(nothing, nothing, x_394);
+  return x_393;
+}
+
+intptr_t fn1_proj1LUL_684(intptr_t* env) {
+  intptr_t A_390; intptr_t B_391; intptr_t __392; intptr_t x_687;
+  A_390 = env[1];
+  B_391 = env[2];
+  __392 = env[3];
+  x_687 = fn0_proj1LUL_683(A_390, B_391, __392);
+  return x_687;
+}
+
+intptr_t fn0_proj1LLU_688(intptr_t A_396, intptr_t B_397, intptr_t __398) {
+  intptr_t x_399; intptr_t x_400; intptr_t x_690;
+  x_690 = appc(__398, 4);
+  x_400 = x_690;
+  x_399 = fn0_sing_elimLL_630(nothing, nothing, x_400);
+  return x_399;
+}
+
+intptr_t fn1_proj1LLU_689(intptr_t* env) {
+  intptr_t A_396; intptr_t B_397; intptr_t __398; intptr_t x_692;
+  A_396 = env[1];
+  B_397 = env[2];
+  __398 = env[3];
+  x_692 = fn0_proj1LLU_688(A_396, B_397, __398);
+  return x_692;
+}
+
+intptr_t fn0_proj1LLL_693(intptr_t A_402, intptr_t B_403, intptr_t __404) {
+  intptr_t x_405; intptr_t x_406; intptr_t x_695;
+  x_695 = appc(__404, 4);
+  ffree(__404);
+  x_406 = x_695;
+  x_405 = fn0_sing_elimLL_630(nothing, nothing, x_406);
+  return x_405;
+}
+
+intptr_t fn1_proj1LLL_694(intptr_t* env) {
+  intptr_t A_402; intptr_t B_403; intptr_t __404; intptr_t x_697;
+  A_402 = env[1];
+  B_403 = env[2];
+  __404 = env[3];
+  x_697 = fn0_proj1LLL_693(A_402, B_403, __404);
+  return x_697;
+}
+
+intptr_t fn0_proj2UUU_698(intptr_t A_408, intptr_t B_409, intptr_t x_410) {
+  intptr_t x_411; intptr_t x_700;
+  x_700 = appc(x_410, 5);
+  x_411 = x_700;
+  return x_411;
+}
+
+intptr_t fn1_proj2UUU_699(intptr_t* env) {
+  intptr_t A_408; intptr_t B_409; intptr_t x_410; intptr_t x_702;
+  A_408 = env[1];
+  B_409 = env[2];
+  x_410 = env[3];
+  x_702 = fn0_proj2UUU_698(A_408, B_409, x_410);
+  return x_702;
+}
+
+intptr_t fn0_proj2UUL_703(intptr_t A_413, intptr_t B_414, intptr_t x_415) {
+  intptr_t x_416; intptr_t x_705;
+  x_705 = appc(x_415, 5);
+  ffree(x_415);
+  x_416 = x_705;
+  return x_416;
+}
+
+intptr_t fn1_proj2UUL_704(intptr_t* env) {
+  intptr_t A_413; intptr_t B_414; intptr_t x_415; intptr_t x_707;
+  A_413 = env[1];
+  B_414 = env[2];
+  x_415 = env[3];
+  x_707 = fn0_proj2UUL_703(A_413, B_414, x_415);
+  return x_707;
+}
+
+intptr_t fn0_proj2ULU_708(intptr_t A_418, intptr_t B_419, intptr_t x_420) {
+  intptr_t x_421; intptr_t x_710;
+  x_710 = appc(x_420, 5);
+  x_421 = x_710;
+  return x_421;
+}
+
+intptr_t fn1_proj2ULU_709(intptr_t* env) {
+  intptr_t A_418; intptr_t B_419; intptr_t x_420; intptr_t x_712;
+  A_418 = env[1];
+  B_419 = env[2];
+  x_420 = env[3];
+  x_712 = fn0_proj2ULU_708(A_418, B_419, x_420);
+  return x_712;
+}
+
+intptr_t fn0_proj2ULL_713(intptr_t A_423, intptr_t B_424, intptr_t x_425) {
+  intptr_t x_426; intptr_t x_715;
+  x_715 = appc(x_425, 5);
+  ffree(x_425);
+  x_426 = x_715;
+  return x_426;
+}
+
+intptr_t fn1_proj2ULL_714(intptr_t* env) {
+  intptr_t A_423; intptr_t B_424; intptr_t x_425; intptr_t x_717;
+  A_423 = env[1];
+  B_424 = env[2];
+  x_425 = env[3];
+  x_717 = fn0_proj2ULL_713(A_423, B_424, x_425);
+  return x_717;
+}
+
+intptr_t fn0_proj2LUU_718(intptr_t A_428, intptr_t B_429, intptr_t x_430) {
+  intptr_t x_431; intptr_t x_720;
+  x_720 = appc(x_430, 5);
+  x_431 = x_720;
+  return x_431;
+}
+
+intptr_t fn1_proj2LUU_719(intptr_t* env) {
+  intptr_t A_428; intptr_t B_429; intptr_t x_430; intptr_t x_722;
+  A_428 = env[1];
+  B_429 = env[2];
+  x_430 = env[3];
+  x_722 = fn0_proj2LUU_718(A_428, B_429, x_430);
+  return x_722;
+}
+
+intptr_t fn0_proj2LUL_723(intptr_t A_433, intptr_t B_434, intptr_t x_435) {
+  intptr_t x_436; intptr_t x_725;
+  x_725 = appc(x_435, 5);
+  ffree(x_435);
+  x_436 = x_725;
+  return x_436;
+}
+
+intptr_t fn1_proj2LUL_724(intptr_t* env) {
+  intptr_t A_433; intptr_t B_434; intptr_t x_435; intptr_t x_727;
+  A_433 = env[1];
+  B_434 = env[2];
+  x_435 = env[3];
+  x_727 = fn0_proj2LUL_723(A_433, B_434, x_435);
+  return x_727;
+}
+
+intptr_t fn0_proj2LLU_728(intptr_t A_438, intptr_t B_439, intptr_t x_440) {
+  intptr_t x_441; intptr_t x_730;
+  x_730 = appc(x_440, 5);
+  x_441 = x_730;
+  return x_441;
+}
+
+intptr_t fn1_proj2LLU_729(intptr_t* env) {
+  intptr_t A_438; intptr_t B_439; intptr_t x_440; intptr_t x_732;
+  A_438 = env[1];
+  B_439 = env[2];
+  x_440 = env[3];
+  x_732 = fn0_proj2LLU_728(A_438, B_439, x_440);
+  return x_732;
+}
+
+intptr_t fn0_proj2LLL_733(intptr_t A_443, intptr_t B_444, intptr_t x_445) {
+  intptr_t x_446; intptr_t x_735;
+  x_735 = appc(x_445, 5);
+  ffree(x_445);
+  x_446 = x_735;
+  return x_446;
+}
+
+intptr_t fn1_proj2LLL_734(intptr_t* env) {
+  intptr_t A_443; intptr_t B_444; intptr_t x_445; intptr_t x_737;
+  A_443 = env[1];
+  B_444 = env[2];
+  x_445 = env[3];
+  x_737 = fn0_proj2LLL_733(A_443, B_444, x_445);
+  return x_737;
+}
+
+intptr_t fn0_my_apair0_738(intptr_t b_448) {
+  intptr_t x_449; intptr_t x_450; intptr_t x_740;
+  switch(b_448){
+    case 4: //true_4
+      x_449 = 6;
+      break;
+    case 5: //false_5
+      x_740 = appc(nat_make_352, 6);
+      x_450 = x_740;
+      x_449 = x_450;
+      break;
+  }
+  return x_449;
+}
+
+intptr_t fn1_my_apair0_739(intptr_t* env) {
+  intptr_t b_448; intptr_t x_742;
+  b_448 = env[1];
+  x_742 = fn0_my_apair0_738(b_448);
+  return x_742;
+}
+
+intptr_t fn1_lam_743(intptr_t* env) {
+  intptr_t free_streamU_326; intptr_t uncons_streamU_336;
+  intptr_t nat_stream_452; intptr_t lam_455; intptr_t b_456; intptr_t x_457;
+  intptr_t x_458; intptr_t x_459; intptr_t m_460; intptr_t n_461;
+  intptr_t __462; intptr_t x_463;
+  lam_455 = env[0];
+  free_streamU_326 = env[1];
+  uncons_streamU_336 = env[2];
+  nat_stream_452 = env[3];
+  b_456 = env[4];
+  switch(b_456){
+    case 4: //true_4
+      x_459 = fn0_uncons_streamU_643(nothing, nat_stream_452);
+      m_460 = getbox(x_459, 0);
+      n_461 = getbox(x_459, 1);
+      x_463 = fn0_free_streamU_633(nothing, n_461);
+      __462 = x_463;
+      x_458 = m_460;
+      ffree(x_459);
+      x_457 = x_458;
+      break;
+    case 5: //false_5
+      x_457 = nat_stream_452;
+      break;
+  }
+  return x_457;
+}
+
+intptr_t fn1_aux_613(intptr_t* env) {
+  intptr_t ord_269; intptr_t chr_272; intptr_t str_275; intptr_t aux_286;
+  intptr_t i_287; intptr_t x_288; intptr_t x_289; intptr_t r_290;
+  intptr_t x_291; intptr_t i_292; intptr_t x_293; intptr_t x_294;
+  intptr_t x_295; intptr_t x_296; intptr_t x_297; intptr_t x_298;
+  intptr_t x_299; intptr_t x_300; intptr_t x_301; intptr_t x_302;
+  intptr_t x_614;
+  aux_286 = env[0];
+  ord_269 = env[1];
+  chr_272 = env[2];
+  str_275 = env[3];
+  i_287 = env[4];
+  x_289 = __lte__(10, i_287);
+  switch(x_289){
+    case 4: //true_4
+      x_291 = __mod__(i_287, 10);
+      r_290 = x_291;
+      x_293 = __div__(i_287, 10);
+      i_292 = x_293;
+      x_614 = appc(aux_286, i_292);
+      x_295 = x_614;
+      x_298 = fn0_ord_599('0');
+      x_297 = __add__(r_290, x_298);
+      x_296 = fn0_chr_602(x_297);
+      x_294 = __push__(x_295, x_296);
+      x_288 = x_294;
+      break;
+    case 5: //false_5
+      x_302 = fn0_ord_599('0');
+      x_301 = __add__(i_287, x_302);
+      x_300 = fn0_chr_602(x_301);
+      x_299 = fn0_str_605(x_300);
+      x_288 = x_299;
+      break;
+  }
+  return x_288;
+}
+
+intptr_t fn1_loop_591(intptr_t* env) {
+  intptr_t x_254; intptr_t m_256; intptr_t loop_259; intptr_t acc_260;
+  intptr_t y_261; intptr_t x_262; intptr_t x_263; intptr_t x_264;
+  intptr_t x_265; intptr_t x_266; intptr_t x_267; intptr_t x_592;
+  intptr_t x_593;
+  loop_259 = env[0];
+  x_254 = env[1];
+  m_256 = env[2];
+  acc_260 = env[3];
+  y_261 = env[4];
+  x_263 = __lte__(y_261, 0);
+  switch(x_263){
+    case 4: //true_4
+      x_262 = acc_260;
+      break;
+    case 5: //false_5
+      x_266 = __mul__(x_254, acc_260);
+      x_265 = __mod__(x_266, m_256);
+      x_267 = __sub__(y_261, 1);
+      x_592 = appc(loop_259, x_265);
+      x_593 = appc(x_592, x_267);
+      x_264 = x_593;
+      x_262 = x_264;
+      break;
+  }
+  return x_262;
+}
+
+intptr_t fn1_loop_581(intptr_t* env) {
+  intptr_t x_240; intptr_t loop_244; intptr_t acc_245; intptr_t y_246;
+  intptr_t x_247; intptr_t x_248; intptr_t x_249; intptr_t x_250;
+  intptr_t x_251; intptr_t x_582; intptr_t x_583;
+  loop_244 = env[0];
+  x_240 = env[1];
+  acc_245 = env[2];
+  y_246 = env[3];
+  x_248 = __lte__(y_246, 0);
+  switch(x_248){
+    case 4: //true_4
+      x_247 = acc_245;
+      break;
+    case 5: //false_5
+      x_250 = __mul__(x_240, acc_245);
+      x_251 = __sub__(y_246, 1);
+      x_582 = appc(loop_244, x_250);
+      x_583 = appc(x_582, x_251);
+      x_249 = x_583;
+      x_247 = x_249;
+      break;
+  }
+  return x_247;
+}
+
+intptr_t fn1_loop_544(intptr_t* env) {
+  intptr_t pred_118; intptr_t sub_131; intptr_t loop_154; intptr_t x_155;
+  intptr_t y_156; intptr_t x_157; intptr_t x_158; intptr_t x_159;
+  intptr_t x_160; intptr_t x_161; intptr_t x_162; intptr_t n_163;
+  intptr_t x_164; intptr_t x_165; intptr_t x_545; intptr_t x_546;
+  loop_154 = env[0];
+  pred_118 = env[1];
+  sub_131 = env[2];
+  x_155 = env[3];
+  y_156 = env[4];
+  x_159 = fn0_pred_530(y_156);
+  x_158 = fn0_sub_536(x_155, x_159);
+  switch(x_158){
+    case 6: //zero_6
+      x_157 = 6;
+      break;
+    default:
+      x_162 = fn0_pred_530(y_156);
+      x_161 = fn0_sub_536(x_155, x_162);
+      n_163 = getbox(x_161, 0);
+      x_545 = appc(loop_154, n_163);
+      x_546 = appc(x_545, y_156);
+      x_164 = x_546;
+      x_165 = mkbox(7, 1); //succ_7
+      setbox(x_165, x_164, 0);
+      x_160 = x_165;
+      x_157 = x_160;
+      break;
+  }
+  return x_157;
+}
+
+int main() {
+  begin_run();
+  intptr_t nat_stream_452; intptr_t x_453; intptr_t x_454; intptr_t x_465;
+  intptr_t x_466; intptr_t x_744;
+  idU_1 = mkclo(fn1_idU_468, 0, 2);
+  idL_4 = mkclo(fn1_idL_471, 0, 2);
+  rwlUU_7 = mkclo(fn1_rwlUU_474, 0, 6);
+  rwlUL_14 = mkclo(fn1_rwlUL_477, 0, 6);
+  rwlLU_21 = mkclo(fn1_rwlLU_480, 0, 6);
+  rwlLL_28 = mkclo(fn1_rwlLL_483, 0, 6);
+  rwrUU_35 = mkclo(fn1_rwrUU_486, 0, 6);
+  rwrUL_42 = mkclo(fn1_rwrUL_489, 0, 6);
+  rwrLU_49 = mkclo(fn1_rwrLU_492, 0, 6);
+  rwrLL_56 = mkclo(fn1_rwrLL_495, 0, 6);
+  sing_elimUU_63 = mkclo(fn1_sing_elimUU_498, 0, 3);
+  sing_elimUL_67 = mkclo(fn1_sing_elimUL_501, 0, 3);
+  sing_elimLU_71 = mkclo(fn1_sing_elimLU_504, 0, 3);
+  sing_elimLL_75 = mkclo(fn1_sing_elimLL_507, 0, 3);
+  not_79 = mkclo(fn1_not_510, 0, 1);
+  and_82 = mkclo(fn1_and_513, 0, 2);
+  or_87 = mkclo(fn1_or_516, 0, 2);
+  xor_92 = mkclo(fn1_xor_519, 0, 2);
+  string_of_bool_98 = mkclo(fn1_string_of_bool_522, 0, 1);
+  lte_103 = mkclo(fn1_lte_525, 0, 2);
+  lt_113 = mkclo(fn1_lt_528, 0, 2);
+  pred_118 = mkclo(fn1_pred_531, 0, 1);
+  add_123 = mkclo(fn1_add_534, 0, 2);
+  sub_131 = mkclo(fn1_sub_537, 0, 2);
+  mul_139 = mkclo(fn1_mul_540, 0, 2);
+  div_147 = mkclo(fn1_div_543, 0, 2);
+  rem_167 = mkclo(fn1_rem_553, 0, 2);
+  rconsUU_173 = mkclo(fn1_rconsUU_556, 0, 3);
+  rconsUL_184 = mkclo(fn1_rconsUL_559, 0, 3);
+  rconsLL_195 = mkclo(fn1_rconsLL_562, 0, 3);
+  free_listUU_206 = mkclo(fn1_free_listUU_565, 0, 3);
+  free_listUL_217 = mkclo(fn1_free_listUL_570, 0, 3);
+  free_listLL_228 = mkclo(fn1_free_listLL_575, 0, 3);
+  pow_239 = mkclo(fn1_pow_580, 0, 2);
+  powm_253 = mkclo(fn1_powm_590, 0, 3);
+  ord_269 = mkclo(fn1_ord_600, 0, 1);
+  chr_272 = mkclo(fn1_chr_603, 0, 1);
+  str_275 = mkclo(fn1_str_606, 0, 1);
+  strlen_279 = mkclo(fn1_strlen_609, 0, 1);
+  string_of_int_282 = mkclo(fn1_string_of_int_612, 0, 1);
+  sing_elimUU_310 = mkclo(fn1_sing_elimUU_622, 0, 3);
+  sing_elimUL_314 = mkclo(fn1_sing_elimUL_625, 0, 3);
+  sing_elimLU_318 = mkclo(fn1_sing_elimLU_628, 0, 3);
+  sing_elimLL_322 = mkclo(fn1_sing_elimLL_631, 0, 3);
+  free_streamU_326 = mkclo(fn1_free_streamU_634, 0, 2);
+  free_streamL_331 = mkclo(fn1_free_streamL_639, 0, 2);
+  uncons_streamU_336 = mkclo(fn1_uncons_streamU_644, 0, 2);
+  uncons_streamL_344 = mkclo(fn1_uncons_streamL_649, 0, 2);
+  nat_make_352 = mkclo(fn1_nat_make_654, 0, 2);
+  proj1UUU_359 = mkclo(fn1_proj1UUU_659, 0, 3);
+  proj1UUL_365 = mkclo(fn1_proj1UUL_664, 0, 3);
+  proj1ULU_371 = mkclo(fn1_proj1ULU_669, 0, 3);
+  proj1ULL_377 = mkclo(fn1_proj1ULL_674, 0, 3);
+  proj1LUU_383 = mkclo(fn1_proj1LUU_679, 0, 3);
+  proj1LUL_389 = mkclo(fn1_proj1LUL_684, 0, 3);
+  proj1LLU_395 = mkclo(fn1_proj1LLU_689, 0, 3);
+  proj1LLL_401 = mkclo(fn1_proj1LLL_694, 0, 3);
+  proj2UUU_407 = mkclo(fn1_proj2UUU_699, 0, 3);
+  proj2UUL_412 = mkclo(fn1_proj2UUL_704, 0, 3);
+  proj2ULU_417 = mkclo(fn1_proj2ULU_709, 0, 3);
+  proj2ULL_422 = mkclo(fn1_proj2ULL_714, 0, 3);
+  proj2LUU_427 = mkclo(fn1_proj2LUU_719, 0, 3);
+  proj2LUL_432 = mkclo(fn1_proj2LUL_724, 0, 3);
+  proj2LLU_437 = mkclo(fn1_proj2LLU_729, 0, 3);
+  proj2LLL_442 = mkclo(fn1_proj2LLL_734, 0, 3);
+  my_apair0_447 = mkclo(fn1_my_apair0_739, 0, 1);
+  x_744 = appc(nat_make_352, 6);
+  x_453 = x_744;
+  nat_stream_452 = x_453;
+  x_454 = mkclo(fn1_lam_743, 3, 1);
+  setclo(x_454, free_streamU_326, 1);
+  setclo(x_454, uncons_streamU_336, 2);
+  setclo(x_454, nat_stream_452, 3);
+  my_apair1_451 = x_454;
+  x_466 = fn0_proj2ULL_713(nothing, nothing, my_apair1_451);
+  x_465 = fn0_free_streamU_633(nothing, x_466);
+  __464 = x_465;
+  end_run();
+}
+
