src/gen/prelude.h
@@ -1,0 +1,11 @@
+#ifndef PRELUDE_H
+#define PRELUDE_H
+
+#define __exU__ 50
+#define __exL__ 48
+#define __tt__ 27
+#define __true__ 4
+#define __false__ 5
+
+#endif
+
