coq/era_inv.v
@@ -66,9 +66,9 @@ Proof. move e:(Box)=>m' ty. elim: ty e=>//{Γ Δ m m' A}. Qed.
 
 Lemma era_lam0_invX Γ Δ A1 A2 A3 B C m1 m2 s1 s2 t l :
   Γ ; Δ ⊢ Lam0 A1 m1 s1 ~ Lam0 A2 m2 s1 : C ->
-  C === Pi0 A3 B s2 ->
+  C ≃ Pi0 A3 B s2 ->
   (A3 :: Γ) ⊢ B : Sort t l ->
-  (A3 :: Γ) ; _: Δ ⊢ m1 ~ m2 : B /\ A1 === A3.
+  (A3 :: Γ) ; _: Δ ⊢ m1 ~ m2 : B /\ A1 ≃ A3.
 Proof with eauto.
   move e1:(Lam0 A1 m1 s1)=>n1.
   move e2:(Lam0 A2 m2 s1)=>n2 tyL.
@@ -90,9 +90,9 @@ Qed.
 
 Lemma era_lam1_invX Γ Δ A1 A2 A3 B C m1 m2 s1 s2 t l :
   Γ ; Δ ⊢ Lam1 A1 m1 s1 ~ Lam1 A2 m2 s1 : C ->
-  C === Pi1 A3 B s2 ->
+  C ≃ Pi1 A3 B s2 ->
   (A3 :: Γ) ⊢ B : Sort t l ->
-  exists r, (A3 :: Γ) ; A3 .{r} Δ ⊢ m1 ~ m2 : B /\ A1 === A3.
+  exists r, (A3 :: Γ) ; A3 .{r} Δ ⊢ m1 ~ m2 : B /\ A1 ≃ A3.
 Proof with eauto.
   move e1:(Lam1 A1 m1 s1)=>n1.
   move e2:(Lam1 A2 m2 s1)=>n2 tyL.
@@ -120,7 +120,7 @@ Qed.
 
 Lemma era_lam0_inv Γ Δ m m' A1 A2 A3 B s1 s2 :
   Γ ; Δ ⊢ Lam0 A1 m s2 ~ Lam0 A2 m' s2 : Pi0 A3 B s1 ->
-  (A3 :: Γ) ; _: Δ ⊢ m ~ m' : B /\ A1 === A3.
+  (A3 :: Γ) ; _: Δ ⊢ m ~ m' : B /\ A1 ≃ A3.
 Proof with eauto.
   move=>ty.
   have[t[l/sta_pi0_inv[r[l1[l2[tyB _]]]]]]:=dyn_valid (era_dyn_type ty).
@@ -129,7 +129,7 @@ Qed.
 
 Lemma era_lam1_inv Γ Δ m m' A1 A2 A3 B s1 s2 :
   Γ ; Δ ⊢ Lam1 A1 m s2 ~ Lam1 A2 m' s2 : Pi1 A3 B s1 ->
-  exists r, (A3 :: Γ) ; A3 .{r} Δ ⊢ m ~ m' : B /\ A1 === A3.
+  exists r, (A3 :: Γ) ; A3 .{r} Δ ⊢ m ~ m' : B /\ A1 ≃ A3.
 Proof with eauto.
   move=>ty.
   have[t[l/sta_pi1_inv[r[l1[l2[tyB _]]]]]]:=dyn_valid (era_dyn_type ty).
@@ -138,7 +138,7 @@ Qed.
 
 Lemma era_pair0_invX Γ Δ A B m m' n n' s r t l C :
   Γ ; Δ ⊢ Pair0 m n s ~ Pair0 m' n' s : C ->
-  C === Sig0 A B r ->
+  C ≃ Sig0 A B r ->
   Γ ⊢ Sig0 A B r : Sort t l ->
   s = r /\ n' = Box /\ Γ ; Δ ⊢ m ~ m' : A /\ Γ ⊢ n : B.[m/].
 Proof with eauto.
@@ -162,7 +162,7 @@ Qed.
 
 Lemma era_pair1_invX Γ Δ A B m m' n n' s r t l C :
   Γ ; Δ ⊢ Pair1 m n s ~ Pair1 m' n' s : C ->
-  C === Sig1 A B r ->
+  C ≃ Sig1 A B r ->
   Γ ⊢ Sig1 A B r : Sort t l ->
   exists Δ1 Δ2,
     Δ1 ∘ Δ2 => Δ /\ s = r /\
