coq/era_subst.v
@@ -31,13 +31,13 @@ Inductive era_agree_subst :
   Γ1 ; Δb ⊢ n ~ n' : A.[σ1] ->
   Γ1 ; Δ1 ⊢ n .: σ1 ~ n' .: σ2 ⊣ (A :: Γ2) ; (A .{s} Δ2)
 | era_agree_subst_conv0 Γ1 Δ1 σ1 σ2 Γ2 Δ2 A B s l :
-  A === B ->
+  A ≃ B ->
   Γ1 ⊢ B.[ren (+1)].[σ1] : Sort s l ->
   Γ2 ⊢ B : Sort s l ->
   Γ1 ; Δ1 ⊢ σ1 ~ σ2 ⊣ (A :: Γ2) ; (_: Δ2) ->
   Γ1 ; Δ1 ⊢ σ1 ~ σ2 ⊣ (B :: Γ2) ; (_: Δ2)
 | era_agree_subst_conv1 Γ1 Δ1 σ1 σ2 Γ2 Δ2 A B s l :
-  A === B ->
+  A ≃ B ->
   Γ1 ⊢ B.[ren (+1)].[σ1] : Sort s l ->
   Γ2 ⊢ B : Sort s l ->
   Γ1 ; Δ1 ⊢ σ1 ~ σ2 ⊣ (A :: Γ2) ; (A .{s} Δ2) ->
@@ -318,7 +318,7 @@ Proof.
 Qed.
 
 Lemma era_ctx_conv0 Γ Δ m m' A B C s l :
-  B === A ->
+  B ≃ A ->
   Γ ⊢ B : Sort s l -> (A :: Γ) ; _: Δ ⊢ m ~ m' : C -> (B :: Γ) ; _: Δ ⊢ m ~ m' : C.
 Proof with eauto using dyn_wf, era_agree_subst_refl.
   move=>eq tyB tym.
@@ -333,7 +333,7 @@ Proof with eauto using dyn_wf, era_agree_subst_refl.
 Qed.
 
 Lemma era_ctx_conv1 Γ Δ m m' A B C s l :
-  B === A ->
+  B ≃ A ->
   Γ ⊢ B : Sort s l -> (A :: Γ) ; A .{s} Δ ⊢ m ~ m' : C -> (B :: Γ) ; B .{s} Δ ⊢ m ~ m' : C.
 Proof with eauto using dyn_wf, era_agree_subst_refl.
   move=>eq tyA tym.
