coq/sta_inv.v
@@ -8,7 +8,7 @@ Unset Printing Implicit Defensive.
 
 Lemma sta_pi0_inv Γ A B C s :
   Γ ⊢ Pi0 A B s : C ->
-  exists t l1 l2, (A :: Γ) ⊢ B : Sort t l1 /\ C === Sort s l2.
+  exists t l1 l2, (A :: Γ) ⊢ B : Sort t l1 /\ C ≃ Sort s l2.
 Proof with eauto.
   move e:(Pi0 A B s)=>m ty.
   elim: ty A B s e=>//{Γ C m}.
@@ -24,7 +24,7 @@ Qed.
 
 Lemma sta_pi1_inv Γ A B C s :
   Γ ⊢ Pi1 A B s : C ->
-  exists t l1 l2, (A :: Γ) ⊢ B : Sort t l1 /\ C === Sort s l2.
+  exists t l1 l2, (A :: Γ) ⊢ B : Sort t l1 /\ C ≃ Sort s l2.
 Proof with eauto.
   move e:(Pi1 A B s)=>m ty.
   elim: ty A B s e=>//{Γ C m}.
@@ -40,7 +40,7 @@ Qed.
 
 Lemma sta_sig0_inv Γ A B C t :
   Γ ⊢ Sig0 A B t : C ->
-  exists s r l1 l2, s ⊑ t /\ Γ ⊢ A : Sort s l1 /\ (A :: Γ) ⊢ B : Sort r l2 /\ C === Sort t (maxn l1 l2).
+  exists s r l1 l2, s ⊑ t /\ Γ ⊢ A : Sort s l1 /\ (A :: Γ) ⊢ B : Sort r l2 /\ C ≃ Sort t (maxn l1 l2).
 Proof with eauto.
   move e:(Sig0 A B t)=>m ty.
   elim: ty A B t e=>//{Γ C m}.
@@ -58,7 +58,7 @@ Lemma sta_sig1_inv Γ A B C t :
   Γ ⊢ Sig1 A B t : C ->
   exists s r l1 l2,
     s ⊑ t /\ r ⊑ t /\
-    Γ ⊢ A : Sort s l1 /\ (A :: Γ) ⊢ B : Sort r l2 /\ C === Sort t (maxn l1 l2).
+    Γ ⊢ A : Sort s l1 /\ (A :: Γ) ⊢ B : Sort r l2 /\ C ≃ Sort t (maxn l1 l2).
 Proof with eauto.
   move e:(Sig1 A B t)=>m ty.
   elim: ty A B t e=>//{Γ C m}.
@@ -74,7 +74,7 @@ Qed.
 
 Lemma sta_ifte_inv Γ m n1 n2 A C :
   Γ ⊢ Ifte A m n1 n2 : C ->
-  A.[m/] === C /\
+  A.[m/] ≃ C /\
   Γ ⊢ m : Bool /\
   Γ ⊢ n1 : A.[TT/] /\
   Γ ⊢ n2 : A.[FF/].
@@ -91,7 +91,7 @@ Qed.
 
 Lemma sta_id_inv Γ A B m n :
   Γ ⊢ Id A m n : B ->
-  exists l, Γ ⊢ m : A /\ Γ ⊢ n : A /\ B === Sort U l.
+  exists l, Γ ⊢ m : A /\ Γ ⊢ n : A /\ B ≃ Sort U l.
 Proof with eauto.
   move e:(Id A m n)=>x tyI.
   elim: tyI A m n e=>//{Γ x B}.
@@ -105,7 +105,7 @@ Proof with eauto.
 Qed.
 
 Lemma sta_lam0_pi1_false Γ A1 A2 B C m s1 s2 :
-  Γ ⊢ Lam0 A1 m s1 : C -> C === Pi1 A2 B s2 -> False.
+  Γ ⊢ Lam0 A1 m s1 : C -> C ≃ Pi1 A2 B s2 -> False.
 Proof with eauto.
   move e:(Lam0 A1 m s1)=>n tyL.
   elim: tyL A1 A2 B m s1 s2 e=>//{Γ C n}.
@@ -116,7 +116,7 @@ Proof with eauto.
 Qed.
 
 Lemma sta_lam1_pi0_false Γ A1 A2 B C m s1 s2 :
-  Γ ⊢ Lam1 A1 m s1 : C -> C === Pi0 A2 B s2 -> False.
+  Γ ⊢ Lam1 A1 m s1 : C -> C ≃ Pi0 A2 B s2 -> False.
 Proof with eauto.
   move e:(Lam1 A1 m s1)=>n tyL.
   elim: tyL A1 A2 B m s1 s2 e=>//{Γ C n}.
@@ -127,7 +127,7 @@ Proof with eauto.
 Qed.
 
 Lemma sta_pair0_sig1_false Γ A B C m1 m2 s1 s2 :
-  Γ ⊢ Pair0 m1 m2 s1 : C -> C === Sig1 A B s2 -> False.
+  Γ ⊢ Pair0 m1 m2 s1 : C -> C ≃ Sig1 A B s2 -> False.
 Proof with eauto.
   move e:(Pair0 m1 m2 s1)=>n tyP.
   elim: tyP A B m1 m2 s1 s2 e=>//{Γ C n}.
@@ -138,7 +138,7 @@ Proof with eauto.
 Qed.
 
 Lemma sta_pair1_sig0_false Γ A B C m1 m2 s1 s2 :
-  Γ ⊢ Pair1 m1 m2 s1 : C -> C === Sig0 A B s2 -> False.
+  Γ ⊢ Pair1 m1 m2 s1 : C -> C ≃ Sig0 A B s2 -> False.
 Proof with eauto.
   move e:(Pair1 m1 m2 s1)=>n tyP.
   elim: tyP A B m1 m2 s1 s2 e=>//{Γ C n}.
